Slicing.dfy
@@ -6,20 +6,19 @@ include "SlideDG.dfy"
 method {:verify false}Slice(S: Statement, V: set<Variable>) returns (slidesSV: set<Slide>)
 	requires Core(S)
 {
-	var cfg := ComputeCFG(S);
-	//var pdgN, pdgE := ComputePDG(S, cfg); // TODO: Change to PDG
-	var slideDG := ComputeSlideDG(S, cfg);
+	var labels := {};
+	var slideDG := ComputeSlideDG(S, labels); //////////////// send labels := labels of S but only Assignment, IF and DO !!!
 
-	slidesSV := ComputeSlice(S, V, slideDG, cfg);
+	slidesSV := ComputeSlice(S, V, slideDG);
 }
 
-/*method {:verify false}ComputeSlice(S: Statement, V: set<Variable>, slideDG: SlideDG, cfg: CFG) returns (slidesSV: set<Slide>)
+/*method {:verify false}ComputeSlice(S: Statement, V: set<Variable>, slideDG: SlideDG) returns (slidesSV: set<Slide>)
 	requires Core(S)
 	requires forall s :: s in SlideDGSlides(slideDG) ==> s in SlideDGMap(slideDG)
 	requires forall s1,s2 :: s1 in SlideDGMap(slideDG) && s2 in SlideDGMap(slideDG)[s1]  ==> s2 in SlideDGSlides(slideDG)
-	ensures forall Sm :: Sm in slidesSV <==> (Sm in finalDefSlides(S, slideDG, cfg, V) || (exists Sn :: Sn in finalDefSlides(S, slideDG, cfg, V) && SlideDGReachable(slideDG, Sm, Sn, SlideDGSlides(slideDG))))	 
+	ensures forall Sm :: Sm in slidesSV <==> (Sm in finalDefSlides(S, slideDG, V) || (exists Sn :: Sn in finalDefSlides(S, slideDG, V) && SlideDGReachable(slideDG, Sm, Sn, SlideDGSlides(slideDG))))	 
 {
-	slidesSV := FindFinalDefSlides(S, slideDG, cfg, V);
+	slidesSV := FindfinalDefSlides(S, slideDG, V);
 	
 	var worklist := slidesSV;
 	var visited := {};
@@ -35,26 +34,26 @@ method {:verify false}Slice(S: Statement, V: set<Variable>) returns (slidesSV: s
 	}
 }*/
 
-method {:verify false}ComputeSlice(S: Statement, V: set<Variable>, slideDG: SlideDG, cfg: CFG) returns (slidesSV: set<Slide>)
+method {:verify false}ComputeSlice(S: Statement, V: set<Variable>, slideDG: SlideDG) returns (slidesSV: set<Slide>)
 	requires Core(S)
 	requires forall s :: s in SlideDGSlides(slideDG) ==> s in SlideDGMap(slideDG)
 	requires forall s1,s2 :: s1 in SlideDGMap(slideDG) && s2 in SlideDGMap(slideDG)[s1]  ==> s2 in SlideDGSlides(slideDG)
-	ensures forall Sm :: Sm in slidesSV <==> (Sm in finalDefSlides(S, slideDG, cfg, V) || (exists Sn :: Sn in finalDefSlides(S, slideDG, cfg, V) && SlideDGReachable(slideDG, Sm, Sn, SlideDGSlides(slideDG))))	 
+	ensures forall Sm :: Sm in slidesSV <==> (Sm in finalDefSlides(S, slideDG, V) || (exists Sn :: Sn in finalDefSlides(S, slideDG, V) && SlideDGReachable(slideDG, Sm, Sn, SlideDGSlides(slideDG))))	 
 {
-	slidesSV := FindFinalDefSlides(S, slideDG, cfg, V);
-	assert slidesSV == finalDefSlides(S, slideDG, cfg, V);
+	slidesSV := FindFinalDefSlides(S, slideDG, V);
+	assert slidesSV == finalDefSlides(S, slideDG, V);
 
 	var worklist := slidesSV;
 
 	var visited := {};
 	
 	while (|worklist| > 0)
-		invariant forall Sm :: Sm in slidesSV <==> (Sm in finalDefSlides(S, slideDG, cfg, V) || (exists Sn :: Sn in visited * finalDefSlides(S, slideDG, cfg, V) && SlideDGReachable(slideDG, Sm, Sn, SlideDGSlides(slideDG))))	 
+		invariant forall Sm :: Sm in slidesSV <==> (Sm in finalDefSlides(S, slideDG, V) || (exists Sn :: Sn in visited * finalDefSlides(S, slideDG, V) && SlideDGReachable(slideDG, Sm, Sn, SlideDGSlides(slideDG))))	 
 		invariant forall Sn :: Sn in worklist ==> Sn in SlideDGMap(slideDG)
 		invariant worklist <= slidesSV <= SlideDGSlides(slideDG)
 		invariant visited + worklist == slidesSV
 		invariant visited * worklist == {}
-		//invariant forall Sm :: Sm in worklist ==> (Sm in finalDefSlides(S, slideDG, cfg, V) || (exists Sn :: Sn in visited * finalDefSlides(S, slideDG, cfg, V) && SlideDGReachable(slideDG, Sm, Sn, SlideDGSlides(slideDG))))
+		//invariant forall Sm :: Sm in worklist ==> (Sm in finalDefSlides(S, slideDG, V) || (exists Sn :: Sn in visited * finalDefSlides(S, slideDG, V) && SlideDGReachable(slideDG, Sm, Sn, SlideDGSlides(slideDG))))
 		decreases SlideDGSlides(slideDG) - visited
 	{
 		var slide :| slide in worklist;
@@ -90,24 +89,24 @@ method {:verify false}ComputeSlice(S: Statement, V: set<Variable>, slideDG: Slid
 		slidesSV := slidesSV + newlyReachable; // + SlideDGMap(slideDG)[slide];
 		worklist := worklist + newlyReachable; // + (SlideDGMap(slideDG)[slide] - visited)
 
-		assert forall Sm :: Sm in slidesSV ==> (Sm in finalDefSlides(S, slideDG, cfg, V) || (exists Sn :: Sn in visited * finalDefSlides(S, slideDG, cfg, V) && SlideDGReachable(slideDG, Sm, Sn, SlideDGSlides(slideDG)))) by {
-			assert forall Sm :: Sm in slidesSV - newlyReachable ==> (Sm in finalDefSlides(S, slideDG, cfg, V) || (exists Sn :: Sn in (visited - {slide}) * finalDefSlides(S, slideDG, cfg, V) && SlideDGReachable(slideDG, Sm, Sn, SlideDGSlides(slideDG))));
+		assert forall Sm :: Sm in slidesSV ==> (Sm in finalDefSlides(S, slideDG, V) || (exists Sn :: Sn in visited * finalDefSlides(S, slideDG, V) && SlideDGReachable(slideDG, Sm, Sn, SlideDGSlides(slideDG)))) by {
+			assert forall Sm :: Sm in slidesSV - newlyReachable ==> (Sm in finalDefSlides(S, slideDG, V) || (exists Sn :: Sn in (visited - {slide}) * finalDefSlides(S, slideDG, V) && SlideDGReachable(slideDG, Sm, Sn, SlideDGSlides(slideDG))));
 			
 		}
-		assert forall Sm :: Sm in slidesSV <== (Sm in finalDefSlides(S, slideDG, cfg, V) || (exists Sn :: Sn in visited * finalDefSlides(S, slideDG, cfg, V) && SlideDGReachable(slideDG, Sm, Sn, SlideDGSlides(slideDG))));	 
+		assert forall Sm :: Sm in slidesSV <== (Sm in finalDefSlides(S, slideDG, V) || (exists Sn :: Sn in visited * finalDefSlides(S, slideDG, V) && SlideDGReachable(slideDG, Sm, Sn, SlideDGSlides(slideDG))));	 
 
 	}
 }
 
-function finalDefSlides(S: Statement, slideDG: SlideDG, cfg: CFG, V: set<Variable>): set<Slide>
+function finalDefSlides(S: Statement, slideDG: SlideDG, V: set<Variable>): set<Slide>
 	requires Core(S)
 {
-	set slide | slide in SlideDGSlides(slideDG) && SlideVariable(slide) in V && slide in finalDefSlidesOfVariable(S, slideDG, cfg, SlideVariable(slide))
+	set slide | slide in SlideDGSlides(slideDG) && SlideVariable(slide) in V && slide in finalDefSlidesOfVariable(S, slideDG, SlideVariable(slide))
 }
 
-method {:verify true}FindFinalDefSlides(S: Statement, slideDG: SlideDG, cfg: CFG, V: set<Variable>) returns (slidesSV: set<Slide>)
+method {:verify true}FindFinalDefSlides(S: Statement, slideDG: SlideDG, V: set<Variable>) returns (slidesSV: set<Slide>)
 	requires Core(S)
-	ensures slidesSV == finalDefSlides(S, slideDG, cfg, V)
+	ensures slidesSV == finalDefSlides(S, slideDG, V)
 {
 	slidesSV := {};
 	var copyV := V;
@@ -118,22 +117,25 @@ method {:verify true}FindFinalDefSlides(S: Statement, slideDG: SlideDG, cfg: CFG
 		var v :| v in copyV;
 		copyV := copyV - {v};
 
-		var Sv := FindFinalDefSlidesOfVariable(S, slideDG, cfg, v);
+		var Sv := FindFinalDefSlidesOfVariable(S, slideDG, v);
 		slidesSV := slidesSV + Sv;
 	}
 
-	assume slidesSV == finalDefSlides(S, slideDG, cfg, V);
+	assume slidesSV == finalDefSlides(S, slideDG, V);
 }
 
-function finalDefSlidesOfVariable(S: Statement, slideDG: SlideDG, cfg: CFG, v: Variable): set<Slide>
+function finalDefSlidesOfVariable(S: Statement, slideDG: SlideDG, v: Variable): set<Slide>
 	requires Core(S)
 {
-	set slide | slide in SlideDGSlides(slideDG) && ReachingDefinition(S, cfg, CFGNode.Exit, SlideCFGNode(slide), v)
+	var rdIn: set<(Variable, Label)> := set v | v in def(S) :: (v, []);
+	var rdOutv := set pair | pair in ReachingDefinitionsOut(S, rdIn) && pair.0 == v;
+	var slides := set pair | pair in rdOutv :: (pair.1, pair.0);
+	set slide | slide in SlideDGSlides(slideDG) && slide in slides
 }
 
-method {:verify false}FindFinalDefSlidesOfVariable(S: Statement, slideDG: SlideDG, cfg: CFG, v: Variable) returns (slidesSv: set<Slide>)
+method {:verify false}FindFinalDefSlidesOfVariable(S: Statement, slideDG: SlideDG, v: Variable) returns (slidesSv: set<Slide>)
 	requires Core(S)
-	ensures slidesSv == finalDefSlidesOfVariable(S, slideDG, cfg, v)
+	ensures slidesSv == finalDefSlidesOfVariable(S, slideDG, v)
 {
 	slidesSv := {};
 	var vDefNodes := findDefNodes(SlideDGStatement(slideDG), SlideDGSlides(slideDG), v); // find all def nodes of v in slideDG
@@ -142,19 +144,16 @@ method {:verify false}FindFinalDefSlidesOfVariable(S: Statement, slideDG: SlideD
 	{
 		var vDefNode :| vDefNode in vDefNodes;
 		vDefNodes := vDefNodes - {vDefNode};
+		var l := SlideLabel(vDefNode);
+		var cfgNode := CFGNode.Node(l);
+		var pathsToExit := findAllPathsToExit(SlideDGStatement(slideDG), cfg, [cfgNode], {}); // foreach node - find all paths to exit (in cfg) - seq of cfg nodes
+		var res := isFinalDefSlide(SlideDGStatement(slideDG), pathsToExit, vDefNode);	      // check if there is at least one path that its only def is in the source node
 
-		match SlideCFGNode(vDefNode) {
-			case Entry =>
-			case Node(l) =>
-				var cfgNode := CFGNode.Node(l);
-				var pathsToExit := findAllPathsToExit(SlideDGStatement(slideDG), cfg, [cfgNode], {}); // foreach node - find all paths to exit (in cfg) - seq of cfg nodes
-				var res := isFinalDefSlide(SlideDGStatement(slideDG), pathsToExit, vDefNode);	      // check if there is at least one path that its only def is in the source node
-
-				if (res)
-				{
-					slidesSv := slidesSv + {vDefNode};
-				}	
-		}
+		if (res)
+		{
+			slidesSv := slidesSv + {vDefNode};
+		}	
+		
 	}
 }
 
