VarSlideDG.dfy
@@ -1,11 +1,11 @@
 include "Definitions.dfy"
 include "Util.dfy"
-include "PDG.dfy"
+include "SlideDG.dfy"
 
 
 // VarSlideDG Definitions:
 datatype VarSlideTag = Phi | Regular
-type VarSlide = (Variable, VarSlideTag, Label)
+type VarSlide = (Variable, VarSlideTag)//, Label) // label removed
 type VarEdge = (VarSlide, VarSlide, set<Variable>)
 type VarSlideDG = (Statement, set<VarSlide>, map<VarSlide, set<VarSlide>>) // map from node to it's predecssors
 
@@ -19,9 +19,20 @@ function method VarSlideTag(s: VarSlide): VarSlideTag
 	s.1
 }
 
-function method VarSlideLabel(s: VarSlide): Label
+function method VarSlideLabels2(S': Statement, s: VarSlide): set<Label>
 {
-	s.2
+	VarSlideLabelsRec(S', s, [])
+}
+
+function method VarSlideLabelsRec(S': Statement, s: VarSlide, l: Label): set<Label>
+{
+	match S' {
+	case Skip =>				{}
+	case Assignment(LHS,RHS) =>	if VarSlideVariable(s) in setOf(LHS) then {l} else {}
+	case SeqComp(S1,S2) =>		VarSlideLabelsRec(S1, s, [1] + l) + VarSlideLabelsRec(S2, s, [2] + l)	
+	case IF(B0,Sthen,Selse) =>	VarSlideLabelsRec(Sthen, s, [1] + l) + VarSlideLabelsRec(Selse, s, [2] + l)	
+	case DO(B,Sloop) =>			VarSlideLabelsRec(Sloop, s, [1] + l)	
+	}
 }
 
 function method VarSlideDGStatement(varSlideDG: VarSlideDG): Statement
@@ -42,6 +53,25 @@ method ComputeVarSlideDG(S: Statement) returns (varSlideDG: VarSlideDG)
 	ensures IsVarSlideDGOf(varSlideDG, S)
 
 predicate IsVarSlideDGOf(varSlideDG: VarSlideDG, S: Statement)
+{
+	varSlideDG == VarSlideDGOf(S)
+}
+
+function VarSlideDGOf(T: Statement): VarSlideDG /// T is in fact S' (SSA)
+	requires Valid(T) && Core(T)
+{
+	var varSlides := varSlidesOf(T, def(T));
+	var m := map s | s in varSlides :: VarSlideDependencePredecessorsOf(s, T);
+
+	(T, varSlides, m)
+}
+
+function VarSlideDependencePredecessorsOf(Sn: VarSlide, T: Statement): set<VarSlide>
+	requires Valid(T) && Core(T)
+	requires Sn in varSlidesOf(T, def(T))
+{
+	set Sm | Sm in varSlidesOf(T, def(T)) && VarSlideDependence(Sm, Sn, T)
+}
 
 /*
 method ComputeVarSlideDG(S: Statement, pdgN: set<PDGNode>, pdgE: set<PDGEdge>) returns (varSlideDG: VarSlideDG)
@@ -63,7 +93,128 @@ method ComputeVarSlideDGEdges(S: Statement, Slides: set<SSASlide>) returns (edge
 
 }*/
 
-function varSlidesOf(S: Statement, V: set<Variable>) : set<VarSlide>
+function varSlidesOf(S': Statement, V: set<Variable>): set<VarSlide>
+	reads *
+	requires Valid(S') && Core(S')
+{
+	//set s | s in slidesOf(S, V) :: VarSlideOf(S, S', s)
+
+	match S'
+	case Skip =>
+		{}	
+	case Assignment(LHS,RHS) =>
+		set v | v in setOf(LHS) :: (v, Regular)
+	case SeqComp(S1,S2) =>
+		if IsDO(S2) then
+			assert IsAssignment(S1);
+			match S1
+			case Assignment(LHS,RHS) => (set v | v in setOf(LHS) :: (v, Phi)) + varSlidesOf(S2, V)
+		else
+			varSlidesOf(S1, V) + varSlidesOf(S2, V)
+	case IF(B0,Sthen,Selse) =>
+		assert IsSeqComp(Sthen);
+		match Sthen
+		case SeqComp(S1,S2) =>
+			assert IsAssignment(S2);
+			match S2
+			case Assignment(LHS,RHS) =>
+				((set v | v in setOf(LHS) :: (v, Phi)) + varSlidesOf(S1, V) +
+				assert IsSeqComp(Selse);
+				match Selse
+				case SeqComp(S1',S2') =>
+					assert IsAssignment(S2');
+					match S2'
+					case Assignment(LHS',RHS') =>
+						(set v | v in setOf(LHS') :: (v, Phi)) + varSlidesOf(S1', V))
+	case DO(B,Sloop) =>	
+		assert IsSeqComp(Sloop);
+		match Sloop
+		case SeqComp(S1,S2) =>
+			assert IsAssignment(S2);
+			match S2
+			case Assignment(LHS,RHS) => (set v | v in setOf(LHS) :: (v, Phi)) + varSlidesOf(S1, V)
+}
+
+
+function {:verify false}VarLabelOfSlide(S: Statement, S': Statement, slide: Slide): Label
+	reads *
+	requires Valid(S)
+	requires Valid(S')
+	requires Core(S)
+	requires Core(S')
+{
+	VarLabelOf(S, S', SlideLabel(slide))
+}
+
+function {:verify false}VarSlideOf(S: Statement, S': Statement, slide: Slide): VarSlide
+	reads *
+	requires Valid(S)
+	requires Valid(S')
+	requires Core(S)
+	requires Core(S')
+{
+	var l := SlideLabel(slide);
+	var varLabel := VarLabelOf(S, S', l);
+	var i := InstanceOf(S', varLabel);
+	(i, Regular)//, varLabel)
+}
+
+function VarLabelOf(S: Statement, S': Statement, l: Label): Label
+	//requires S == RemoveEmptyAssignments(Rename(S', XLs, X))
+	reads *
+	requires Valid(S)
+	requires Valid(S')
+	requires Core(S)
+	requires Core(S')
+	requires ValidLabel(l, S)
+	//ensures |VarLabelOf(S, S', l)| >= 1 && |VarLabelOf(S, S', l)| <= maxLabelSize(S')
+	ensures ValidLabel(VarLabelOf(S, S', l), S')
+{
+	match S {
+	case Skip =>				assume IsSkip(S');
+								assert l == [];
+								[]	
+	case Assignment(LHS,RHS) =>	assume IsAssignment(S');
+								assert l == [];
+								[]
+	case SeqComp(S1,S2) =>		if l == [] then [] else
+								assume IsSeqComp(S');
+								match S' {
+								case SeqComp(S1',S2') => if l[0] == 1 then [1] + VarLabelOf(S1, S1', l[1..]) else [2] + VarLabelOf(S2, S2', l[1..])
+								}	
+	case IF(B0,Sthen,Selse) =>	if l == [] then [] else
+								assume IsIF(S');
+								match S' {							
+								case IF(B0',Sthen',Selse') => if l[0] == 1 then [1,1] + VarLabelOf(Sthen, Sthen', l[1..]) else [2,1] + VarLabelOf(Selse, Selse', l[1..])
+								}
+	case DO(B,Sloop) =>			if l == [] then [2] else
+								assume IsSeqComp(S');
+								match S' {
+								// S1' is the phi assignment and S2' is the DO
+								// we should add another [2] in order to go to the loop
+								case SeqComp(S1',S2') => assume IsDO(S2');
+														 match S2' {
+														 case DO(B',Sloop') => assume Valid(Sloop') && Core(Sloop'); [2,1,1] + VarLabelOf(Sloop, Sloop', l[1..])
+														 }
+								}
+	}
+}
+
+function {:verify false}InstanceOf(S': Statement, varLabel: Label): Variable
+/////////////////////////// Should add v: Variable to the function and return LHS' * vsSSA.getInstancesOf(v).
+	reads *
+	requires Valid(S')
+	requires Core(S')
+	//requires |varLabel| >= 1 && |varLabel| <= maxLabelSize(S')
+{
+	match S' {
+	case Skip =>					""
+	case Assignment(LHS',RHS') =>	assume |LHS'| >= 1; LHS'[0]
+	case SeqComp(S1',S2') =>		if varLabel[0] == 1 then InstanceOf(S1', varLabel[1..]) else InstanceOf(S2', varLabel[1..])
+	case IF(B0',Sthen',Selse') =>	""//if varLabel[0] == 1 then InstanceOf(Sthen', varLabel[1..]) else InstanceOf(Selse', varLabel[1..])
+	case DO(B',Sloop') =>			""//InstanceOf(Sloop', varLabel[1..])
+	}
+}
 
 datatype VarSlideDGPath = Empty | Extend(VarSlideDGPath, VarSlide)
 
@@ -115,6 +266,11 @@ predicate VarSlideDGReachableVia(varSlideDG: VarSlideDG, from: VarSlide, via: Va
 }
 
 function VarSlideDGNeighbours(varSlideDG: VarSlideDG, n: VarSlide) : set<VarSlide>
+	requires n in VarSlideDGMap(varSlideDG)
+{
+	VarSlideDGMap(varSlideDG)[n]
+}
+
 
 predicate VarSlideDGReachablePhi(varSlideDG: VarSlideDG, from: VarSlide, to: VarSlide, S: set<VarSlide>)
 	//requires null !in S
@@ -136,9 +292,19 @@ predicate VarSlideDGReachableViaPhi(varSlideDG: VarSlideDG, from: VarSlide, via:
 
 ////////// VarSlide Dependence: ////////////
 
-predicate VarSlideDependence(m: VarSlide, n: VarSlide, S: Statement)
+predicate VarSlideDependence(Sm: VarSlide, Sn: VarSlide, S: Statement) // S is S'
 	reads *
 	requires Valid(S) && Core(S)
 {
-	VarSlideVariable(m) in UsedVars(S, VarSlideLabel(n))
+	var v := VarSlideVariable(Sm);
+	exists l :: l in VarSlideLabels(Sn, S) && 
+	v in UsedVars(S, l)
+}
+
+function VarSlideLabels(s: VarSlide, S: Statement): set<Label>
+	requires Valid(S) && Core(S)
+	requires s in varSlidesOf(S, def(S))
+{
+	set l | l == VarSlideLabel(s) ||
+	(l < VarSlideLabel(s) && (IsDO(slipOf(S, l)) || IsIF(slipOf(S, l))))
 }
